proof/refine/ARM/Syscall_R.thy
@@ -1111,7 +1111,7 @@ lemma get_mrs_length_rv[wp]:
 lemma st_tcb_at_idle_thread':
   "\<lbrakk> st_tcb_at' P (ksIdleThread s) s; valid_idle' s \<rbrakk>
         \<Longrightarrow> P IdleThreadState"
-  by (clarsimp simp: valid_idle'_def pred_tcb_at'_def obj_at'_def)
+  by (clarsimp simp: valid_idle'_def pred_tcb_at'_def obj_at'_def idle_tcb'_def)
 
 crunch tcb_at'[wp]: replyFromKernel "tcb_at' t"
 
@@ -1306,7 +1306,7 @@ lemma hinv_invs'[wp]:
          apply (subgoal_tac "thread \<noteq> ksIdleThread s", simp_all)[1]
           apply (fastforce elim!: pred_tcb'_weakenE st_tcb_ex_cap'')
          apply (clarsimp simp: valid_idle'_def valid_state'_def
-                               invs'_def pred_tcb_at'_def obj_at'_def)
+                               invs'_def pred_tcb_at'_def obj_at'_def idle_tcb'_def)
         apply wp+
        apply (rule_tac Q="\<lambda>rv'. invs' and valid_invocation' rv
                                 and (\<lambda>s. ksSchedulerAction s = ResumeCurrentThread)
@@ -1785,7 +1785,7 @@ proof
   assume "ksCurThread s = ksIdleThread s"
   with vi have "ct_in_state' idle' s"
     unfolding ct_in_state'_def valid_idle'_def
-    by (clarsimp simp: pred_tcb_at'_def obj_at'_def)
+    by (clarsimp simp: pred_tcb_at'_def obj_at'_def idle_tcb'_def)
 
   with cts show False
     unfolding ct_in_state'_def
